begin typed

Semantics/Imp/Typed/Aexp.lean
@@ -1,75 +1,18 @@
-import Semantics.Imp.Untyped.Syntax
+import Semantics.Imp.Typed.Lang
 
 namespace Aexp
+namespace Natural
 
 -- Operational semantics of aexp
-inductive Natural: Aexp × State → Val → Prop
-  | num₁:
-    Natural (num n, _) n
+inductive Step: Aexp → State → Val → Prop
+  | val: Step (val n) _ n
+  | var: Step (var x) s v
+  | addₙ
+    (h₁: Step a s $ Val.nat n) (h₂: Step b s $ Val.nat m):
+    Step (add a b) s (Val.nat $ n + m)
+  | addᵢ
+    (h₁: Step a s (Val.int n)) (h₂: Step b s (Val.int m)):
+    Step (add a b) s (Val.int $ n + m)
 
-  | loc₁:
-    Natural (loc x, s) (s x)
-
-  | add₁ (h₁: Natural (a,s) n) (h₂: Natural (b,s) m):
-    Natural (add a b, s) (n + m)
-
-  | sub₁ (h₁: Natural (a,s) n) (h₂: Natural (b,s) m):
-    Natural (sub a b, s) (n - m)
-
-  | mul₁ (h₁: Natural (a,s) n) (h₂: Natural (b,s) m):
-    Natural (mul a b, s) (n * m)
-
-infix:110 " ⟹ " => Natural
-
--- Denotational semantics of arithmetic expressions
-@[reducible]
-def reduce (a: Aexp) (s: State): Val :=
-  match a with
-  | num n => n
-  | loc x => s x
-  | add a b => reduce a s + reduce b s
-  | sub a b => reduce a s - reduce b s
-  | mul a b => reduce a s * reduce b s
-
-infix:110 "⇓" => reduce
-
--- relational definition is equal to recursive
-theorem reduce.from_natural (h: as ⟹ n): reduce.uncurry as = n :=
-  by induction h with
-  | num₁ => rfl
-  | loc₁ => rfl
-  | _ _ _ ih₁ ih₂ => exact ih₁ ▸ ih₂ ▸ rfl
-
-theorem Natural.from_reduce {a: Aexp} (h: a⇓s = n): (a,s) ⟹ n :=
-  by induction a generalizing n with
-  | num _ => exact h ▸ num₁
-  | loc _ => exact h ▸ loc₁
-  | add _ _ l r => exact h ▸ add₁ (l rfl) (r rfl)
-  | sub _ _ l r => exact h ▸ sub₁ (l rfl) (r rfl)
-  | mul _ _ l r => exact h ▸ mul₁ (l rfl) (r rfl)
-
-@[simp] theorem Natural_iff_reduce: (a, s) ⟹ n ↔ a⇓s = n := ⟨reduce.from_natural, Natural.from_reduce⟩
-@[simp] theorem Natural_iff_reduce': (a, s) ⟹ (a⇓s) := Natural.from_reduce rfl
-
-protected instance Natural.equiv: Setoid Aexp where
-  r a b := ∀ s n, (a, s) ⟹ n = (b, s) ⟹ n
-  iseqv := {
-    refl := λ _ _ _ ↦ Eq.refl _
-    symm := λ h s n ↦ Eq.symm (h s n)
-    trans := λ h₁ h₂ x n ↦ (h₁ x n) ▸ (h₂ x n)
-  }
-
-instance reduce.equiv: Setoid Aexp where
-  r a b := ∀s, a⇓s = b⇓s
-  iseqv := ⟨λ _ _ ↦ Eq.refl _, (Eq.symm $ · ·) , λ h₁ h₂ s ↦ (h₁ s) ▸ (h₂ s)⟩
-
-protected theorem Natural_eq_eq_reduce_eq: Natural.equiv.r a b ↔ reduce.equiv.r a b := by
-  constructor <;> intro h
-  . simp [Setoid.r] at *
-    intro s
-    specialize h s
-    exact h
-  . simp [Setoid.r] at *
-    simp [h]
-
+end Natural
 end Aexp
