Semantics/Imp/Typed/Bexp.lean
@@ -1,89 +1,26 @@
-import Semantics.Imp.Untyped.Aexp
+import Semantics.Imp.Typed.Aexp
 
 namespace Bexp
+namespace Natural
 
 -- Operational semantics of Bexp
-inductive Natural: Bexp × State → Bool → Prop
-  | tt₁:
-    Natural (tt, _) true
+inductive Step: Bexp → State → Bool → Prop
+  | tt: Step tt _ true
+  | ff: Step ff _ false
+  | leₙ
+    (h₁: Aexp.Natural.Step a s (Val.nat n))
+    (h₂: Aexp.Natural.Step b s (Val.nat m)):
+    Step (le a b) s (n ≤ m)
+  | leᵢ
+    (h₁: Aexp.Natural.Step a s (Val.int n))
+    (h₂: Aexp.Natural.Step b s (Val.int m)):
+    Step (le a b) s (n ≤ m)
+  | not
+    (h: Step a s n):
+    Step (not a) s (!n)
+  | and
+    (h₁: Step a s n) (h₂: Step b s m):
+    Step (and a b) s (n && m)
 
-  | ff₁:
-    Natural (ff, _) false
-
-  | eq₁:
-    Natural (eq a b, s) (a⇓s = b⇓s)
-
-  | le₁:
-    Natural (le a b, s) (a⇓s ≤ b⇓s)
-
-  | not₁ {a: Bexp} (h: Natural (a,s) n):
-    Natural (not a, s) (!n)
-
-  | and₁ {a b: Bexp} (h₁: Natural (a,s) n) (h₂: Natural (b,s) m):
-    Natural (and a b, s) (n && m)
-
-  | or₁ {a b: Bexp} (h₁: Natural (a,s) n) (h₂: Natural (b,s) m):
-    Natural (or a b, s) (n || m)
-
-infix:110 " ⟹ " => Natural
-
--- Denotational semantics of Bexp
-@[reducible, simp] def reduce (b: Bexp) (s: State): Bool :=
-  match b with
-  | tt      => true
-  | ff      => false
-  | not b   => !reduce b s
-  | and a b => reduce a s && reduce b s
-  | or a b  => reduce a s || reduce b s
-  | eq a b  => a⇓s = b⇓s
-  | le a b  => a⇓s ≤ b⇓s
-
-infix:110 "⇓" => reduce
-
--- relational definition is equivalent to recursive
-theorem Natural.from_reduce {b: Bexp} (h: b⇓s = x): (b, s) ⟹ x :=
-  by induction b generalizing x with
-  | tt => exact h ▸ Natural.tt₁
-  | ff => exact h ▸ Natural.ff₁
-  | eq => exact h ▸ Natural.eq₁
-  | le => exact h ▸ Natural.le₁
-  | not _ ih => exact h ▸ Natural.not₁ (ih rfl)
-  | and _ _ l r => exact h ▸ Natural.and₁ (l rfl) (r rfl)
-  | or _ _  l r => exact h ▸ Natural.or₁  (l rfl) (r rfl)
-
-theorem reduce.from_natural {bs: Bexp × State} (h: bs ⟹ x): reduce.uncurry bs = x :=
-  by induction h with
-  | tt₁ => rfl
-  | ff₁ => rfl
-  | eq₁ => rfl
-  | le₁ => rfl
-  | not₁ _ ih => exact ih ▸ rfl
-  | _ _ _ ih₁ ih₂ => exact ih₁ ▸ ih₂ ▸ rfl
-
-@[simp] theorem Natural_eq_reduce {b: Bexp}: (b,s) ⟹ r ↔ b⇓s = r := ⟨reduce.from_natural, Natural.from_reduce⟩
-
-theorem not_true_eq_false: (!b⇓s) = (not b)⇓s := by simp
-
-protected instance Natural.equiv: Setoid Bexp where
-  r a b := ∀ s n, (a, s) ⟹ n = (b, s) ⟹ n
-  iseqv := {
-    refl := λ _ _ _ ↦ Eq.refl _
-    symm := λ h s n ↦ Eq.symm (h s n)
-    trans := λ h₁ h₂ x n ↦ (h₁ x n) ▸ (h₂ x n)
-  }
-
-@[reducible, simp]
-instance reduce.equiv: Setoid Bexp where
-  r a b:= ∀s, a⇓s = b⇓s
-  iseqv := ⟨λ _ _ ↦ Eq.refl _, (Eq.symm $ · ·) , λ h₁ h₂ s ↦ (h₁ s) ▸ (h₂ s)⟩
-
-protected theorem Natural_eq_eq_reduce_eq: Natural.equiv.r a b ↔ reduce.equiv.r a b := by
-  constructor <;> intro h
-  . simp [Setoid.r] at *
-    intro s
-    specialize h s
-    exact h
-  . simp [Setoid.r] at *
-    simp [h]
-
+end Natural
 end Bexp
