Semantics/Imp/Typed/Structural.lean
@@ -6,9 +6,9 @@ namespace Com
 namespace Structural
 
 @[reducible]
-inductive Step: Config → Config → Prop where
-  | ass₁:
-    Step (ass x a, s) (skip, s⟪x ≔ a⇓s⟫)
+inductive Step: Com × State → Com × State → Prop where
+  | ass (h: Aexp.Natural.Step a s n):
+    Step (ass x a, s) (skip, s⟪x ≔ n⟫)
 
   | cat₁:
     Step (skip;;c, s) (c, s)
@@ -16,19 +16,19 @@ inductive Step: Config → Config → Prop where
   | cat₂ (h: Step (c, s) (e, t)):
     Step (c;;d, s) (e;;d, t)
 
-  | cond₁:
-    Step (cond b c d, s) (bif b⇓s then c else d, s)
+  | cond (h: Bexp.Natural.Step b s t):
+    Step (cond b c d, s) (bif t then c else d, s)
 
-  | loop₁:
-    Step (loop b c, s) (bif b⇓s then c;;loop b c else skip, s)
+  | loop (h: Bexp.Natural.Step b s t):
+    Step (loop b c, s) (bif t then c;;loop b c else skip, s)
 
 infix:110 " ⇒ " => Step
 
 theorem Step.demo₁:
-  (⦃x = 2; while 0 <= x {x = x - 1}⦄, ⟪⟫) ⇒
-      (⦃skip; while 0 <= x {x = x - 1}⦄, ⟪⟫⟪"x"≔2⟫) := cat₂ ass₁
+  (⦃x = 0; while x <= 2 {x = x + 1}⦄, ⟪⟫) ⇒
+      (⦃skip; while x <= 2 {x = x + 1}⦄, ⟪⟫⟪"x"≔0⟫) := cat₂ (ass (by simp))
 
-@[simp] theorem Step.cat_iff:
+@[simp] theorem cat_iff:
   (c₁;;c₂, s) ⇒ et ↔
   (∃e t, (c₁, s) ⇒ (e, t) ∧ et = (e;;c₂, t))
   ∨ (c₁ = skip ∧ et = (c₂, s)) := by
@@ -45,7 +45,7 @@ theorem Step.demo₁:
       cases h with | intro h₁ h₂ =>
         exact h₁ ▸ h₂ ▸ Step.cat₁
 
-@[simp] lemma Step.cond_iff:
+@[simp] lemma cond_iff:
   (cond b c d, s) ⇒ ss ↔
   (b⇓s ∧ ss = (c, s)) ∨ (b⇓s = false ∧ ss = (d, s)) := by
   constructor <;> intro h
@@ -54,46 +54,34 @@ theorem Step.demo₁:
     . exact Or.inl ⟨rfl, hb ▸ rfl⟩
   . have hss: ss = (bif b⇓s then c else d, s) := by
       cases hb: b⇓s <;> rw [hb] at h <;> simp at * <;> assumption
-    exact hss ▸ Step.cond₁
+    exact hss ▸ Step.cond
 
-@[simp] lemma Step.cond_false {b: Bexp} (hb: b⇓s = false):
+@[simp] lemma cond_false {b: Bexp} (hb: b⇓s = false):
   (cond b c d, s) ⇒ ss ↔ (ss = (d, s)) :=
   by rw [cond_iff, hb]; simp
 
-open Relation
+infix:110 " ⇒* " => Relation.ReflTransGen Step
 
-namespace Star
+theorem Star.demo₂:
+  (⦃x = 2; while 0 <= x {x = x + 1}⦄, ⟪⟫) ⇒*
+      (⦃while 0 <= x {x = x + 1}⦄, ⟪⟫⟪"x"≔2⟫) :=
+  Relation.ReflTransGen.head (Step.cat₂ Step.ass) (Relation.ReflTransGen.head Step.cat₁ Relation.ReflTransGen.refl)
 
-alias head   := ReflTransGen.head
-alias trans  := ReflTransGen.trans
-alias refl   := ReflTransGen.refl
-alias single := ReflTransGen.single
-alias lift   := ReflTransGen.lift
-alias head_induction_on := ReflTransGen.head_induction_on
-
-infix:110 " ⇒* " => ReflTransGen Step
-
-theorem demo₂:
-  (⦃x = 2; while 0 <= x {x = x - 1}⦄, ⟪⟫) ⇒*
-      (⦃while 0 <= x {x = x - 1}⦄, ⟪⟫⟪"x"≔2⟫) :=
-  head (Step.cat₂ Step.ass₁) (head Step.cat₁ Star.refl)
-
-theorem cat_skip_cat
+theorem Star.cat_skip_cat
   (h: (c, s) ⇒* (skip, t)):
   (c;;d, s) ⇒* (skip;;d, t) :=
-  lift (λ (x: Config) ↦ (x.1;;d, x.2)) (λ _ _ h => Step.cat₂ h) h
+  Relation.ReflTransGen.lift (λ (x: Com × State) ↦ (x.1;;d, x.2)) (λ _ _ h => Step.cat₂ h) h
 
-theorem cat
+theorem Star.cat
   (h₁: (c₁, s) ⇒* (skip, s₁))
   (h₂: (c₂, s₁) ⇒* (skip, s₂)):
   (c₁;;c₂, s) ⇒* (skip, s₂) :=
-  trans (cat_skip_cat h₁) (trans (single Step.cat₁) h₂)
+  Relation.ReflTransGen.trans (cat_skip_cat h₁) (Relation.ReflTransGen.trans (Relation.ReflTransGen.single Step.cat₁) h₂)
 
-theorem cat_no_influence
+theorem Star.cat_no_influence
   (h: (c₁, s) ⇒* (skip, s₁)):
   (c₁;;c₂, s) ⇒* (c₂, s₁) :=
-  trans (cat_skip_cat h) (single Step.cat₁)
+  Relation.ReflTransGen.trans (cat_skip_cat h) (Relation.ReflTransGen.single Step.cat₁)
 
-end Star
 end Structural
 end Com
