Semantics/Imp/Untyped/Aexp.lean
@@ -1,26 +1,15 @@
-import Semantics.Imp.Untyped.Syntax
+import Semantics.Imp.Untyped.Lang
 
 namespace Aexp
 namespace Natural
 
 -- Operational semantics of aexp
-inductive Step: Aexp × State → Val → Prop
-  | val₁:
-    Step (val n, _) n
-
-  | loc₁:
-    Step (loc x, s) (s x)
-
-  | add₁ (h₁: Step (a, s) n) (h₂: Step (b, s) m):
-    Step (add a b, s) (n + m)
-
-  | sub₁ (h₁: Step (a, s) n) (h₂: Step (b, s) m):
-    Step (sub a b, s) (n - m)
-
-  | mul₁ (h₁: Step (a, s) n) (h₂: Step (b, s) m):
-    Step (mul a b, s) (n * m)
-
-infix:110 " ⟹ " => Step
+inductive Step: Aexp → State → Val → Prop
+  | val: Step (val n) _ n
+  | var: Step (var x) s (s x)
+  | add
+    (h₁: Step a s n) (h₂: Step b s m):
+    Step (add a b) s (n + m)
 
 end Natural
 
@@ -29,33 +18,26 @@ end Natural
 def reduce (a: Aexp) (s: State): Val :=
   match a with
   | val n => n
-  | loc x => s x
+  | var x => s x
   | add a b => reduce a s + reduce b s
-  | sub a b => reduce a s - reduce b s
-  | mul a b => reduce a s * reduce b s
-
-infix:110 "⇓" => reduce
 
 -- relational definition is equal to recursive
-theorem reduce.from_natural (h: as ⟹ n): reduce.uncurry as = n :=
+theorem reduce.from_natural (h: Natural.Step a s n): reduce a s = n :=
   by induction h with
-  | val₁ => rfl
-  | loc₁ => rfl
-  | _ _ _ ih₁ ih₂ => exact ih₁ ▸ ih₂ ▸ rfl
+  | add _ _ ih₁ ih₂ => exact ih₁ ▸ ih₂ ▸ rfl
+  | _ => rfl
 
-theorem Natural.from_reduce {a: Aexp} (h: a⇓s = n): (a,s) ⟹ n :=
+theorem Natural.from_reduce {a: Aexp} (h: reduce a s = n): Step a s n :=
   by induction a generalizing n with
-  | val _ => exact h ▸ Step.val₁
-  | loc _ => exact h ▸ Step.loc₁
-  | add _ _ l r => exact h ▸ Step.add₁ (l rfl) (r rfl)
-  | sub _ _ l r => exact h ▸ Step.sub₁ (l rfl) (r rfl)
-  | mul _ _ l r => exact h ▸ Step.mul₁ (l rfl) (r rfl)
+  | val _ => exact h ▸ Step.val
+  | var _ => exact h ▸ Step.var
+  | add _ _ l r => exact h ▸ Step.add (l rfl) (r rfl)
 
-@[simp] theorem Step_iff_reduce: (a, s) ⟹ n ↔ a⇓s = n := ⟨reduce.from_natural, Natural.from_reduce⟩
-@[simp] theorem Step_iff_reduce': (a, s) ⟹ (a⇓s) := Natural.from_reduce rfl
+@[simp] theorem Step_iff_reduce: Natural.Step a s n ↔ reduce a s = n := ⟨reduce.from_natural, Natural.from_reduce⟩
+@[simp] theorem Step_iff_reduce': Natural.Step a s (reduce a s) := Natural.from_reduce rfl
 
 protected instance Step.equiv: Setoid Aexp where
-  r a b := ∀ s n, (a, s) ⟹ n = (b, s) ⟹ n
+  r a b := ∀ s n, Natural.Step a s n = Natural.Step b s n
   iseqv := {
     refl := λ _ _ _ ↦ Eq.refl _
     symm := λ h s n ↦ Eq.symm (h s n)
@@ -63,7 +45,7 @@ protected instance Step.equiv: Setoid Aexp where
   }
 
 instance reduce.equiv: Setoid Aexp where
-  r a b := ∀s, a⇓s = b⇓s
+  r a b := ∀s, reduce a s = reduce b s
   iseqv := ⟨λ _ _ ↦ Eq.refl _, (Eq.symm $ · ·) , λ h₁ h₂ s ↦ (h₁ s) ▸ (h₂ s)⟩
 
 protected theorem Step_eq_eq_reduce_eq: Step.equiv.r a b ↔ reduce.equiv.r a b := by
