Semantics/Imp/Untyped/Bexp.lean
@@ -4,29 +4,16 @@ namespace Bexp
 namespace Natural
 
 -- Operational semantics of Bexp
-inductive Step: Bexp × State → Bool → Prop
-  | tt₁:
-    Step (tt, _) true
-
-  | ff₁:
-    Step (ff, _) false
-
-  | eq₁:
-    Step (eq a b, s) (a⇓s = b⇓s)
-
-  | le₁:
-    Step (le a b, s) (a⇓s ≤ b⇓s)
-
-  | not₁ {a: Bexp} (h: Step (a,s) n):
-    Step (not a, s) (!n)
-
-  | and₁ {a b: Bexp} (h₁: Step (a,s) n) (h₂: Step (b,s) m):
-    Step (and a b, s) (n && m)
-
-  | or₁ {a b: Bexp} (h₁: Step (a,s) n) (h₂: Step (b,s) m):
-    Step (or a b, s) (n || m)
-
-infix:110 " ⟹ " => Step
+inductive Step: Bexp → State → Bool → Prop
+  | tt: Step tt _ true
+  | ff: Step ff _ false
+  | le: Step (le a b) s (a.reduce s ≤ b.reduce s)
+  | not
+    (h: Step a s n):
+    Step (not a) s (!n)
+  | and
+    (h₁: Step a s n) (h₂: Step b s m):
+    Step (and a b) s (n && m)
 
 end Natural
 
@@ -37,38 +24,29 @@ end Natural
   | ff      => false
   | not b   => !reduce b s
   | and a b => reduce a s && reduce b s
-  | or a b  => reduce a s || reduce b s
-  | eq a b  => a⇓s = b⇓s
-  | le a b  => a⇓s ≤ b⇓s
-
-infix:110 "⇓" => reduce
+  | le a b  => a.reduce s ≤ b.reduce s
 
 -- relational definition is equivalent to recursive
-theorem Natural.from_reduce {b: Bexp} (h: b⇓s = x): (b, s) ⟹ x :=
+theorem Natural.from_reduce {b: Bexp} (h: b.reduce s = x): Step b s x :=
   by induction b generalizing x with
-  | tt => exact h ▸ Step.tt₁
-  | ff => exact h ▸ Step.ff₁
-  | eq => exact h ▸ Step.eq₁
-  | le => exact h ▸ Step.le₁
-  | not _ ih => exact h ▸ Step.not₁ (ih rfl)
-  | and _ _ l r => exact h ▸ Step.and₁ (l rfl) (r rfl)
-  | or _ _  l r => exact h ▸ Step.or₁  (l rfl) (r rfl)
+  | tt => exact h ▸ Step.tt
+  | ff => exact h ▸ Step.ff
+  | le => exact h ▸ Step.le
+  | not _ ih => exact h ▸ Step.not (ih rfl)
+  | and _ _ l r => exact h ▸ Step.and (l rfl) (r rfl)
 
-theorem reduce.from_natural {bs: Bexp × State} (h: bs ⟹ x): reduce.uncurry bs = x :=
+theorem reduce.from_natural (h: Natural.Step b s x): reduce b s = x :=
   by induction h with
-  | tt₁ => rfl
-  | ff₁ => rfl
-  | eq₁ => rfl
-  | le₁ => rfl
-  | not₁ _ ih => exact ih ▸ rfl
-  | _ _ _ ih₁ ih₂ => exact ih₁ ▸ ih₂ ▸ rfl
+  | not _ ih => exact ih ▸ rfl
+  | and _ _ ih₁ ih₂ => exact ih₁ ▸ ih₂ ▸ rfl
+  | _ => rfl
 
-@[simp] theorem Step_eq_reduce {b: Bexp}: (b,s) ⟹ r ↔ b⇓s = r := ⟨reduce.from_natural, Natural.from_reduce⟩
+@[simp] theorem Step_eq_reduce {b: Bexp}: Natural.Step b s r ↔ reduce b s = r := ⟨reduce.from_natural, Natural.from_reduce⟩
 
-theorem not_true_eq_false: (!b⇓s) = (not b)⇓s := by simp
+theorem not_true_eq_false: (!b.reduce s) = (not b).reduce s := by simp
 
 protected instance Step.equiv: Setoid Bexp where
-  r a b := ∀ s n, (a, s) ⟹ n = (b, s) ⟹ n
+  r a b := ∀ s n, Natural.Step a s n = Natural.Step b s n
   iseqv := {
     refl := λ _ _ _ ↦ Eq.refl _
     symm := λ h s n ↦ Eq.symm (h s n)
@@ -77,7 +55,7 @@ protected instance Step.equiv: Setoid Bexp where
 
 @[reducible, simp]
 instance reduce.equiv: Setoid Bexp where
-  r a b:= ∀s, a⇓s = b⇓s
+  r a b:= ∀s, a.reduce s = b.reduce s
   iseqv := ⟨λ _ _ ↦ Eq.refl _, (Eq.symm $ · ·) , λ h₁ h₂ s ↦ (h₁ s) ▸ (h₂ s)⟩
 
 protected theorem Step_eq_eq_reduce_eq: Step.equiv.r a b ↔ reduce.equiv.r a b := by
