Semantics/Imp/Untyped/Lang.lean
@@ -1,22 +1,30 @@
-import Semantics.State
+import Mathlib.Logic.Function.Basic
 
 @[reducible]
 def Val := Int
 
+def State := String → Val
+def State.nil: State := λ _ ↦ 0
+
+notation "⟪⟫" => State.nil
+notation s "⟪" x "≔" e "⟫" => Function.update s x e
+
+#reduce ⟪⟫ "x"
+#reduce (⟪⟫⟪"x" ≔ 3⟫⟪"x" ≔ 4⟫) "x"
+#reduce (⟪⟫⟪"x" ≔ 3⟫⟪"x" ≔ 4⟫⟪"x" ≔ 7⟫) "x"
+
+theorem State.demo₁: (⟪⟫⟪"x"≔3⟫) = (⟪⟫⟪"x"≔4⟫⟪"x"≔3⟫) := by simp
+
 inductive Aexp where
   | val : Val → Aexp
-  | loc : String → Aexp
+  | var : String → Aexp
   | add : Aexp → Aexp → Aexp
-  | sub : Aexp → Aexp → Aexp
-  | mul : Aexp → Aexp → Aexp
 
 inductive Bexp where
   | tt
   | ff
   | not : Bexp → Bexp
   | and : Bexp → Bexp → Bexp
-  | or  : Bexp → Bexp → Bexp
-  | eq  : Aexp → Aexp → Bexp
   | le  : Aexp → Aexp → Bexp
 
 inductive Com where
@@ -35,16 +43,12 @@ declare_syntax_cat imp
 -- general
 syntax "(" imp ")" : imp
 -- imp
-syntax num : imp
+syntax num: imp
 syntax ident: imp
 syntax:60 imp:60 "+" imp:61 : imp
-syntax:60 imp:60 "-" imp:61 : imp
-syntax:70 imp:70 "*" imp:71 : imp
 -- bexp
 syntax:80 "!" imp:81 : imp
-syntax:70 imp:70 "==" imp:71 : imp
 syntax:70 imp:70 "<=" imp:71 : imp
-syntax:65 imp:65 "||" imp:66 : imp
 syntax:65 imp:65 "&&" imp:66 : imp
 -- stmt
 syntax:50 imp:50 "=" imp:51 : imp
@@ -58,22 +62,18 @@ syntax "⦃" imp "⦄" : term
 macro_rules
   -- keywords
   | `(⦃skip⦄) => `(Com.skip)
-  | `(⦃true⦄)   => `(Bexp.tt)
-  | `(⦃false⦄)   => `(Bexp.ff)
+  | `(⦃true⦄) => `(Bexp.tt)
+  | `(⦃false⦄) => `(Bexp.ff)
   -- general
   | `(⦃($x)⦄) => `(⦃$x⦄)
   -- imp
-  | `(⦃$x:ident⦄) => `(Aexp.loc $(Lean.quote (toString x.getId)))
+  | `(⦃$x:ident⦄) => `(Aexp.var $(Lean.quote (toString x.getId)))
   | `(⦃$n:num⦄)   => `(Aexp.val $n)
   | `(⦃$x + $y⦄)  => `(Aexp.add ⦃$x⦄ ⦃$y⦄)
-  | `(⦃$x - $y⦄)  => `(Aexp.sub ⦃$x⦄ ⦃$y⦄)
-  | `(⦃$x * $y⦄)  => `(Aexp.mul ⦃$x⦄ ⦃$y⦄)
   -- bexp
   | `(⦃!$x⦄)      => `(Bexp.not ⦃$x⦄)
-  | `(⦃$x == $y⦄)  => `(Bexp.eq ⦃$x⦄ ⦃$y⦄)
   | `(⦃$x <= $y⦄)  => `(Bexp.le ⦃$x⦄ ⦃$y⦄)
   | `(⦃$x && $y⦄)  => `(Bexp.and ⦃$x⦄ ⦃$y⦄)
-  | `(⦃$x || $y⦄)  => `(Bexp.or ⦃$x⦄ ⦃$y⦄)
   -- stmt
   | `(⦃$x:ident = $y⦄) => `(Com.ass $(Lean.quote (toString x.getId)) ⦃$y⦄)
   | `(⦃$x ; $y⦄)       => `(Com.cat ⦃$x⦄ ⦃$y⦄)
@@ -85,5 +85,5 @@ macro_rules
 #check ⦃skip⦄
 #check ⦃x = 5⦄
 #check ⦃x = 5; y = 6⦄
-#check ⦃if x == 5 {y = 6} else {z = 7}⦄
-#check ⦃x = 0; while !(x == 5) {skip; skip; x = x + 1}⦄
+#check ⦃if x <= 5 {y = 6} else {z = 7}⦄
+#check ⦃x = 0; while !(x <= 5) {skip; skip; x = x + 1}⦄
