Semantics/Imp/Untyped/Natural.lean
@@ -4,39 +4,39 @@ namespace Com
 namespace Natural
 
 inductive Step: Com × State → State → Prop
-  | skip₁:
+  | skip:
     Step (skip, s) s
 
-  | ass₁:
-    Step (ass x a, s) (s⟪x ≔ a⇓s⟫)
+  | ass:
+    Step (ass x a, s) (s⟪x ≔ a.reduce s⟫)
 
-  | cat₁ t
+  | cat t
     (hc: Step (c, s) t) (hd: Step (d, t) u):
     Step (c;;d, s) u
 
   | cond₁ {b: Bexp}
-    (hb: b⇓s = true) (hc: Step (c, s) t):
+    (hb: b.reduce s = true) (hc: Step (c, s) t):
     Step (cond b c d, s) t
 
   | cond₂ {b: Bexp}
-    (hb: b⇓s = false) (hd: Step (d, s) t):
+    (hb: b.reduce s = false) (hd: Step (d, s) t):
     Step (cond b c d, s) t
 
   | loop₁ {b: Bexp} u
-    (hb: b⇓s = true) (hc: Step (c, s) u) (hw: Step (loop b c, u) t):
+    (hb: b.reduce s = true) (hc: Step (c, s) u) (hw: Step (loop b c, u) t):
     Step (loop b c, s) t
 
   | loop₂ {b: Bexp}
-    (hb: b⇓s = false):
+    (hb: b.reduce s = false):
     Step (loop b c, s) s
 
 infix:110 " ⟹ " => Step
 
-theorem demo₁: (⦃x = 5⦄, ⟪⟫) ⟹ ⟪⟫⟪"x"≔5⟫ := Step.ass₁
+theorem demo₁: (⦃x = 5⦄, ⟪⟫) ⟹ ⟪⟫⟪"x"≔5⟫ := Step.ass
 
 theorem demo₂:
   (⦃x = 2; if x <= 1 {y = 3} else {z = 4}⦄, ⟪⟫) ⟹
-  (⟪⟫⟪"x"≔2⟫⟪"z"≔4⟫) := Step.cat₁ _ Step.ass₁ $ Step.cond₂ rfl Step.ass₁
+  (⟪⟫⟪"x"≔2⟫⟪"z"≔4⟫) := Step.cat _ Step.ass $ Step.cond₂ rfl Step.ass
 
 /-
 ## Rewriting rules
@@ -45,36 +45,36 @@ theorem demo₂:
 theorem skip_iff: (skip, s) ⟹ t ↔ s = t := by
   apply Iff.intro <;> intro h
   . cases h; rfl
-  . exact h ▸ Step.skip₁
+  . exact h ▸ Step.skip
 
 theorem cat_iff: (c;;d, s) ⟹ t ↔ ∃ w, (c, s) ⟹ w ∧ (d, w) ⟹ t := by
   apply Iff.intro <;> intro h
-  . cases h with | cat₁ t h₁ h₂ =>
+  . cases h with | cat t h₁ h₂ =>
       exact ⟨t, ⟨h₁, h₂⟩⟩
   . cases h with | intro w h =>
-      exact Step.cat₁ w h.1 h.2
+      exact Step.cat w h.1 h.2
 
-theorem cond_iff: (cond b c d, s) ⟹ t ↔ bif b⇓s then (c, s) ⟹ t else (d, s) ⟹ t := by
+theorem cond_iff: (cond b c d, s) ⟹ t ↔ bif b.reduce s then (c, s) ⟹ t else (d, s) ⟹ t := by
   constructor <;> intro h
   . cases h with
     | cond₁ hb hc => exact hb ▸ hc
     | cond₂ hb hc => exact hb ▸ hc
-  . cases hb: b⇓s with
+  . cases hb: b.reduce s with
     | true => exact Step.cond₁ hb $ (cond_true ((c, s) ⟹ t) _) ▸ hb ▸ h
     | false => exact Step.cond₂ hb $ (cond_false _ ((d, s) ⟹ t)) ▸ hb ▸ h
 
-theorem cond_iff': (cond b c d, s) ⟹ t ↔ (bif b⇓s then c else d, s) ⟹ t := by
-  rw [cond_iff]; cases b⇓s <;> simp
+theorem cond_iff': (cond b c d, s) ⟹ t ↔ (bif b.reduce s then c else d, s) ⟹ t := by
+  rw [cond_iff]; cases b.reduce s <;> simp
 
 theorem loop_iff: (loop b c, s) ⟹ t ↔
-  (bif b⇓s then ∃ w, (c, s) ⟹ w ∧ (loop b c, w) ⟹ t else s = t) := by
+  (bif b.reduce s then ∃ w, (c, s) ⟹ w ∧ (loop b c, w) ⟹ t else s = t) := by
   apply Iff.intro <;> intro h
   . cases h with
     | loop₁ t hb hc hw =>
       exact hb ▸ ⟨t, ⟨hc, hw⟩⟩
     | loop₂ hb =>
       exact hb ▸ rfl
-  . cases hb: b⇓s with
+  . cases hb: b.reduce s with
     | true =>
       rw [hb] at h
       cases h with | intro w h =>
@@ -97,16 +97,16 @@ instance equiv: Setoid Com where
 theorem skipl: (skip;;c) ≈ c := by
   intro _ _
   constructor
-  . intro h; cases h with | cat₁ _ hc hd =>
+  . intro h; cases h with | cat _ hc hd =>
       exact skip_iff.mp hc ▸ hd
-  . exact (Step.cat₁ _ Step.skip₁ ·)
+  . exact (Step.cat _ Step.skip ·)
 
 theorem skipr: (c;;skip) ≈ c := by
   intro _ _
   constructor
-  . intro h; cases h with | cat₁ _ hc hd =>
+  . intro h; cases h with | cat _ hc hd =>
       exact skip_iff.mp hd ▸ hc
-  . exact (Step.cat₁ _ · Step.skip₁)
+  . exact (Step.cat _ · Step.skip)
 
 theorem cond_true (h: b ≈ Bexp.tt): cond b c d ≈ c := by
   intro _ _
@@ -124,11 +124,11 @@ theorem loop_unfold:
   constructor <;> intro h
   . rw [cond_iff]
     cases h with
-    | loop₁ w hb hc hw => exact hb ▸ Step.cat₁ w hc hw
-    | loop₂ hb => exact hb ▸ Step.skip₁
+    | loop₁ w hb hc hw => exact hb ▸ Step.cat w hc hw
+    | loop₂ hb => exact hb ▸ Step.skip
   . rw [loop_iff]
     rw [cond_iff] at h
-    cases hb: b⇓s <;> rw [hb] at h
+    cases hb: b.reduce s <;> rw [hb] at h
     . exact skip_iff.mp h
     . exact cat_iff.mp h
 
@@ -151,8 +151,8 @@ theorem loop_tt (h: b ≈ Bexp.tt):
 
 theorem determinist {x: Com × State} (h₁: x ⟹ s) (h₂: x ⟹ t): s = t :=
   by induction h₁ generalizing t with
-  | cat₁ _ _ _ ih₁ ih₂ => cases h₂ with
-    | cat₁ _ hc hd => exact ih₂ (ih₁ hc ▸ hd)
+  | cat _ _ _ ih₁ ih₂ => cases h₂ with
+    | cat _ hc hd => exact ih₂ (ih₁ hc ▸ hd)
 
   | cond₁ hb _ ih => cases h₂ with
     | cond₁ _ hd => exact ih hd
