Semantics/Stlc/Natural.lean
@@ -1,12 +1,13 @@
 import Semantics.Stlc.Syntax
+import Mathlib.Logic.Relation
 
 namespace Term
 namespace Natural
 
 inductive Value: Term → Prop where
-  | abs₁: Value (abs _ _ _)
-  | true₁: Value true
-  | false₁: Value false
+  | abs: Value (abs _ _ _)
+  | true: Value true
+  | false: Value false
 
 def subst (x: String) (s: Term) (t: Term): Term :=
   match t with
@@ -15,6 +16,34 @@ def subst (x: String) (s: Term) (t: Term): Term :=
   | app t₁ t₂ => app (subst x s t₁) (subst x s t₂)
   | cond t₁ t₂ t₃ => cond (subst x s t₁) (subst x s t₂) (subst x s t₃)
   | otherwise => otherwise
+
+notation "[" x "≔" s "]" t => subst x s t
+
+inductive Step: Term → Term → Prop where
+  | appabs (h: Value v):
+    Step (app (abs x _ t) v) ([x ≔ v]t)
+
+  | app₁ (h₁: Step t t'):
+    Step (app t u) (app t' u)
+
+  | app₂ (h₁: Value v) (h₂: Step u u'):
+    Step (app v u) (app v u')
+
+  | cond₁:
+    Step (cond true t _) t
+
+  | cond₂:
+    Step (cond false _ u) u
+
+  | cond₃ (h: Step b b'):
+    Step (cond b t u) (cond b' t u)
+
+infix:100 "⇒" => Step
+
+infix:110 " ⇒* " => Relation.ReflTransGen Step
+
+
+
 
 end Natural
 end Term
